src/SepCancel.v
@@ -33,10 +33,50 @@ Module Make (U : SynUnifier) (SH : SepHeap).
       : option (U.Subst types) :=
       Folds.fold_left_3_opt 
         (fun l r t (acc : U.Subst _) =>
-          if Prove Prover summ (Expr.Equal t l r)
+          if Prove Prover summ (Expr.Equal t (U.exprInstantiate sub l) (U.exprInstantiate sub r))
             then Some acc
             else U.exprUnify bound l r acc)
         l r ts sub.
+
+    Parameter WellTyped_exprInstantiate : forall U G e t S,
+      is_well_typed funcs U G e t = true <-> is_well_typed funcs U G (U.exprInstantiate S e) t = true.
+
+    Lemma unifyArgsOk : forall U G bound summ l r ts R f S S',
+      Valid Prover_correct U G summ ->
+      all2 (@is_well_typed _ funcs U G) l ts = true ->
+      all2 (@is_well_typed _ funcs U G) r ts = true ->
+      unifyArgs bound summ l r ts S = Some S' ->
+      @applyD types (exprD funcs U G) ts (map (U.exprInstantiate S') l) R f =
+      @applyD types (exprD funcs U G) ts (map (U.exprInstantiate S') r) R f /\
+      U.Subst_Extends S' S.
+    Proof.
+      unfold unifyArgs; induction l; destruct r; destruct ts; simpl; intros; try congruence.
+      { inversion H2. split; reflexivity. }
+      { repeat match goal with
+                 | [ H : (if ?X then _ else _) = true |- _ ] =>
+                   revert H; case_eq X; intros; [ | congruence ]
+                 | [ |- context [ exprD ?A ?B ?C ?D ?E ] ] =>
+                   case_eq (exprD A B C D E); intros
+               end; simpl in *;
+        try solve [ 
+          match goal with
+            | [ H : is_well_typed _ _ _ ?e _ = true , H' : exprD _ _ _ (U.exprInstantiate ?S' ?e) _ = None |- _ ] =>
+              exfalso; revert H; revert H'; clear; intros H' H;
+              eapply WellTyped_exprInstantiate with (S := S') in H;
+              eapply is_well_typed_correct in H;
+              rewrite H' in H ; destruct H; congruence
+          end ].
+        revert H2. case_eq (Prove Prover summ (Equal t (U.exprInstantiate S a) (U.exprInstantiate S e))); intros.
+        { eapply Prove_correct in H2; eauto.
+          assert (Provable funcs U G (Equal t (U.exprInstantiate S a) (U.exprInstantiate S e))). eapply H2.
+          unfold ValidProp. simpl. admit. (** TODO: still wrong **)
+          unfold Provable in H8. simpl in H8.
+          admit. }
+        { clear H2. revert H7.
+          case_eq (U.exprUnify bound a e S); intros; try congruence.
+          admit.
+        } }
+    Qed.
 
     Fixpoint unify_remove (bound : nat) (summ : Facts Prover) (l : exprs types) (ts : list tvar) (r : list (exprs types))
       (sub : U.Subst types)
@@ -53,6 +93,15 @@ Module Make (U : SynUnifier) (SH : SepHeap).
               | Some sub => Some (b, sub)
             end
         end.
+
+    Lemma unify_removeOk : forall U G cs bound summ f l ts r r' S S' P,
+      unify_remove bound summ l ts r S = Some (r', S') ->
+      SE.heq funcs preds U G cs
+        (SE.Star (SE.Func f l) P) (SH.starred (SE.Func f) r Emp) ->
+      SE.heq funcs preds U G cs P (SH.starred (SE.Func f) r' Emp) /\
+      U.Subst_Extends S' S.
+    Proof.
+    Admitted.      
 
     Require Ordering.
 
@@ -86,7 +135,7 @@ Module Make (U : SynUnifier) (SH : SepHeap).
       end.
 
     Definition order_impures (imps : MM.mmap (exprs types)) : cancel_list :=
-      MM.FM.fold (fun k => fold_left (fun (acc : cancel_list) (args : exprs types) => 
+      FM.fold (fun k => fold_left (fun (acc : cancel_list) (args : exprs types) => 
         Ordering.insert_in_order _ meta_order_funcs (args, k) acc)) imps nil.
 
     Lemma impuresD'_flatten : forall U G cs imps,
@@ -125,8 +174,8 @@ Module Make (U : SynUnifier) (SH : SepHeap).
       Permutation.Permutation
       (FM.fold (fun (f : FM.key) (argss : list (exprs types)) (acc : list (exprs types * FM.key)) =>
         map (fun args : exprs types => (args, f)) argss ++ acc) imps L)
-      (MM.FM.fold
-        (fun k : MM.FM.key =>
+      (FM.fold
+        (fun k : FM.key =>
          fold_left
            (fun (acc : cancel_list) (args : exprs types) =>
             Ordering.insert_in_order (exprs types * nat) meta_order_funcs
@@ -160,7 +209,7 @@ Module Make (U : SynUnifier) (SH : SepHeap).
       match ls with
         | nil => (acc, rem, sub)
         | (args,f) :: ls => 
-          match MM.FM.find f rem with
+          match FM.find f rem with
             | None => cancel_in_order bound summ ls (MM.mmap_add f args acc) rem sub
             | Some argss =>
               match nth_error preds f with
@@ -169,30 +218,274 @@ Module Make (U : SynUnifier) (SH : SepHeap).
                   match unify_remove bound summ args (SDomain ts) argss sub with
                     | None => cancel_in_order bound summ ls (MM.mmap_add f args acc) rem sub
                     | Some (rem', sub) =>
-                      cancel_in_order bound summ ls acc (MM.FM.add f rem' rem) sub
+                      cancel_in_order bound summ ls acc (FM.add f rem' rem) sub
                   end
               end                      
           end
       end.
+    
+    Definition sheapInstantiate (s : U.Subst types) : MM.mmap (exprs types) -> MM.mmap (exprs types) :=
+      MM.mmap_map (map (@U.exprInstantiate _ s)).
 
-    (** TODO: This isn't quite correct b/c it doesn't understand the fact
-     ** that unification could pin down certain values in U
-     **)
+    Lemma sheapInstantiate_mmap_add : forall U G cs S n e acc,
+      heq funcs preds U G cs
+        (SH.impuresD pcType stateType 
+          (sheapInstantiate S (MM.mmap_add n e acc)))
+        (SH.impuresD pcType stateType 
+          (MM.mmap_add n (map (@U.exprInstantiate _ S) e) 
+                         (sheapInstantiate S acc))).
+    Proof.
+      clear. intros. eapply MM.PROPS.map_induction with (m := acc); intros.
+      { unfold MM.mmap_add, sheapInstantiate, MM.mmap_map.
+        repeat rewrite MF.find_Empty by auto using MF.map_Empty.
+        rewrite SH.impuresD_Equiv. reflexivity.
+        rewrite MF.map_add. simpl.
+        reflexivity. }
+      { unfold MM.mmap_add, sheapInstantiate, MM.mmap_map.
+        rewrite MF.FACTS.map_o. simpl in *. unfold exprs in *. case_eq (FM.find n m'); simpl; intros.
+        { rewrite SH.impuresD_Equiv. reflexivity.
+          rewrite MF.map_add. reflexivity. }
+        { rewrite SH.impuresD_Equiv. reflexivity.
+          rewrite MF.map_add. simpl. reflexivity. } }
+    Qed.
+
+    Lemma sheapInstantiate_Equiv : forall S a b,
+      MM.mmap_Equiv a b ->
+      MM.mmap_Equiv (sheapInstantiate S a) (sheapInstantiate S b).
+    Proof.
+      clear. unfold sheapInstantiate, MM.mmap_Equiv, MM.mmap_map, FM.Equiv; intuition;
+      try solve [ repeat match goal with
+                           | [ H : FM.In _ (FM.map _ _) |- _ ] => apply MF.FACTS.map_in_iff in H
+                           | [ |- FM.In _ (FM.map _ _) ] => apply MF.FACTS.map_in_iff
+                         end; firstorder ].
+      repeat match goal with
+               | [ H : FM.MapsTo _ _ (FM.map _ _) |- _ ] =>
+                 apply MF.FACTS.map_mapsto_iff in H; destruct H; intuition; subst
+             end.
+      apply Permutation.Permutation_map. firstorder.
+    Qed.
+
+    Lemma cancel_in_order_equiv : forall bound summ ls acc rem sub L R S acc',
+      MM.mmap_Equiv acc acc' ->
+      cancel_in_order bound summ ls acc rem sub = (L, R, S) ->
+      exists L' R' S',
+        cancel_in_order bound summ ls acc' rem sub = (L', R', S') /\
+        MM.mmap_Equiv L L' /\
+        MM.mmap_Equiv R R' /\
+        U.Subst_Equal S S'.
+    Proof.
+      clear. induction ls; simpl; intros.
+      { inversion H0; subst; auto. 
+        do 3 eexists. split; [ reflexivity | intuition ]. }
+      { repeat match goal with
+                 | [ H : match ?X with 
+                           | (_,_) => _
+                         end = _ |- _ ] => destruct X
+                 | [ H : match ?X with
+                           | Some _ => _ | None => _ 
+                         end = _ |- _ ] =>
+                 revert H; case_eq X; intros
+                 
+               end;
+        (eapply IHls; [ eauto using MM.mmap_add_mor | eassumption ]). }
+    Qed.
+
+    Lemma cancel_in_order_mmap_add_acc : forall bound summ ls n e acc rem sub L R S,
+      cancel_in_order bound summ ls (MM.mmap_add n e acc) rem sub = (L, R, S) ->
+      exists L' R' S',
+        cancel_in_order bound summ ls acc rem sub = (L', R', S') /\
+        MM.mmap_Equiv (MM.mmap_add n e L') L /\
+        MM.mmap_Equiv R R' /\
+        U.Subst_Equal S S'.
+    Proof.
+      clear. induction ls; simpl; intros.
+      { inversion H; subst. do 3 eexists; split. 
+        reflexivity. split; try reflexivity. split; try reflexivity. }
+      { repeat match goal with
+                 | [ H : match ?X with 
+                           | (_,_) => _
+                         end = _ |- _ ] => destruct X
+                 | [ H : match ?X with
+                           | Some _ => _ | None => _ 
+                         end = _ |- _ ] =>
+                 revert H; case_eq X; intros
+                 
+               end;
+        try solve [ eapply IHls; eauto ];
+        match goal with
+          | [ H : cancel_in_order _ _ _ _ _ _ = _ |- _ ] =>
+            eapply cancel_in_order_equiv in H; [ | eapply MM.mmap_add_comm ]
+        end;
+        repeat match goal with
+                 | [ H : exists x, _ |- _ ] => destruct H
+                 | [ H : _ /\ _ |- _ ] => destruct H
+               end;
+        match goal with
+          | [ H : cancel_in_order _ _ _ _ _ _ = _ |- _ ] =>
+            eapply IHls in H
+        end;
+        repeat match goal with
+                 | [ H : exists x, _ |- _ ] => destruct H
+                 | [ H : _ /\ _ |- _ ] => destruct H
+                 | [ |- exists x, _ /\ _ ] => eexists; split; [ eassumption | ]
+                 | [ |- exists x, _ ] => eexists
+                 | [ H : MM.mmap_Equiv _ _ |- _ ] => rewrite H
+                 | [ H : U.Subst_Equal _ _ |- _ ] => rewrite H
+               end; intuition reflexivity. }
+    Qed.
+
+(*
+    Lemma cancel_in_order_add_acc : forall bound summ ls n e acc rem sub L R S,
+      ~FM.In n acc ->
+      cancel_in_order bound summ ls (FM.add n e acc) rem sub = (L, R, S) ->
+      exists L' R' S',
+        cancel_in_order bound summ ls acc rem sub = (L', R', S') /\
+        MM.mmap_Equiv (FM.add n e L') L /\
+        MM.mmap_Equiv R R' /\
+        U.Subst_Equal S S'.
+    Proof.
+      clear. induction ls; simpl; intros.
+      { inversion H0; subst. do 3 eexists; split. 
+        reflexivity. split; try reflexivity. split; try reflexivity. }
+      { repeat match goal with
+                 | [ H : match ?X with 
+                           | (_,_) => _
+                         end = _ |- _ ] => destruct X
+                 | [ H : match ?X with
+                           | Some _ => _ | None => _ 
+                         end = _ |- _ ] =>
+                 revert H; case_eq X; intros
+                 
+               end;
+        try solve [ eapply IHls; eauto |
+        match goal with
+          | [ H : cancel_in_order _ _ _ _ _ _ = _ |- _ ] =>
+            eapply cancel_in_order_equiv in H; [ | eapply MM.mmap_add_comm ]
+        end;
+        repeat match goal with
+                 | [ H : exists x, _ |- _ ] => destruct H
+                 | [ H : _ /\ _ |- _ ] => destruct H
+               end;
+        match goal with
+          | [ H : cancel_in_order _ _ _ _ _ _ = _ |- _ ] =>
+            eapply IHls in H
+        end;
+        repeat match goal with
+                 | [ H : exists x, _ |- _ ] => destruct H
+                 | [ H : _ /\ _ |- _ ] => destruct H
+                 | [ |- exists x, _ /\ _ ] => eexists; split; [ eassumption | ]
+                 | [ |- exists x, _ ] => eexists
+                 | [ H : MM.mmap_Equiv _ _ |- _ ] => rewrite H
+                 | [ H : U.Subst_Equal _ _ |- _ ] => rewrite H
+               end; intuition reflexivity ].
+        Focus 3.
+        match goal with
+          | [ H : cancel_in_order _ _ _ _ _ _ = _ |- _ ] =>
+            eapply cancel_in_order_equiv in H; [ | ]
+        end.
+        repeat match goal with
+                 | [ H : exists x, _ |- _ ] => destruct H
+                 | [ H : _ /\ _ |- _ ] => destruct H
+               end;
+        match goal with
+          | [ H : cancel_in_order _ _ _ _ _ _ = _ |- _ ] =>
+            eapply IHls in H
+        end.
+
+
+
+ }
+    Qed.
+*)
+
+    Lemma sheapInstantiate_add : forall U G cs S n e acc,
+      heq funcs preds U G cs
+        (SH.impuresD pcType stateType (sheapInstantiate S (FM.add n e acc)))
+        (SH.starred (fun v => Func n (map (U.exprInstantiate S) v)) e
+          (SH.impuresD pcType stateType (sheapInstantiate S (FM.remove n acc)))).
+    Proof.
+      clear. intros.
+        unfold sheapInstantiate, MM.mmap_map.
+    Admitted.
+
     Lemma cancel_in_orderOk : forall U G cs bound summ ls acc rem sub L R S,
       cancel_in_order bound summ ls acc rem sub = (L, R, S) ->
-      himp funcs preds U G cs (SH.impuresD _ _ R) (SH.impuresD _ _ L) ->
       himp funcs preds U G cs 
-        (SH.impuresD _ _ acc)
-        (Star (SH.starred (fun v => (Func (snd v) (fst v))) ls Emp)
-              (SH.impuresD _ _ acc)).
+        (SH.impuresD _ _ (sheapInstantiate S R))
+        (SH.impuresD _ _ (sheapInstantiate S L)) ->
+      himp funcs preds U G cs 
+        (SH.impuresD _ _ (sheapInstantiate S rem))
+        (Star (SH.starred (fun v => (Func (snd v) (map (@U.exprInstantiate _ S) (fst v)))) ls Emp)
+              (SH.impuresD _ _ (sheapInstantiate S acc))).
     Proof.
+      induction ls; simpl; intros.
+      { inversion H; clear H; subst.
+        rewrite SH.starred_def. simpl. heq_canceler. auto. }
+      { repeat match goal with
+                 | [ H : match ?X with 
+                           | (_,_) => _
+                         end = _ |- _ ] => destruct X
+                 | [ H : match ?X with
+                           | Some _ => _ | None => _ 
+                         end = _ |- _ ] =>
+                 revert H; case_eq X; intros
+               end.
+        { eapply IHls in H3; eauto.
+          rewrite SH.impuresD_Equiv.
+          2: eapply sheapInstantiate_Equiv.
+          2: eapply MF.equiv_eq_mor.
+          2: reflexivity. 3: reflexivity. 2: symmetry. 2: apply MF.MapsTo_add_remove_Equal.
+          2: eapply MF.FACTS.find_mapsto_iff; eauto.
+          
+(*
+          rewrite sheapInstantiate_add in H3.
+          rewrite sheapInstantiate_add.
+
+        eapply cancel_in_order_mmap_add_acc in H3.
+        rewrite IHls. 2: 
+        
+
+destruct a. 
+        revert H. case_eq (FM.find n rem).
+        { admit. }
+        { intros.
+
+
+    eapply IHls in H; destruct H; intuition; subst. eexists.
+
+    eapply IHls in H1; destruct H1; intuition; subst.
+    eapply IHls in H.
+  
+
+
+etransitivity. 
+          rewrite IHls.
+
+
+          rewrite sheapInstantiate_mmap_add in H1.
+          SearchAbout SH.impuresD.
+
+
+          Lemma impuresD_mmap_add : forall
+    (U G : env types)
+    (cs : codeSpec (tvarD types pcType) (tvarD types stateType)) 
+    f args
+    (i : FM.t (list (exprs types))),
+  SH.SE.heq funcs preds U G cs 
+    (SH.impuresD pcType stateType (MM.mmap_add f args i))
+    (SH.SE.Star (SH.SE.Func f args)
+       (SH.impuresD pcType stateType i)).
+          Proof.
+          Admitted.
+          rewrite impuresD_mmap_add in H1.
+*)
     Admitted.
 
 
     Definition sepCancel (bound : nat) (summ : Facts Prover) (l r : SH.SHeap types pcType stateType) :
       SH.SHeap _ _ _ * SH.SHeap _ _ _ * U.Subst types :=
       let ordered_r := order_impures (SH.impures r) in
-      let sorted_l := MM.FM.map (fun v => Ordering.sort _ meta_order_args v) (SH.impures l) in 
+      let sorted_l := FM.map (fun v => Ordering.sort _ meta_order_args v) (SH.impures l) in 
       let '(rf, lf, sub) := 
         cancel_in_order bound summ ordered_r (MM.empty _) sorted_l (U.Subst_empty _)
       in
